src/BasicProg.v
@@ -43,8 +43,7 @@ Proof.
   unfold corr2, exis; intros; repeat deex.
   repeat ( apply sep_star_lift2and in H; destruct H ).
   unfold lift in *; simpl in *.
-  remember (Read a rx) as p. generalize dependent Heqp.
-  induction H0; intros; inversion Heqp; subst.
+  inv_exec.
   - apply sep_star_comm in H; apply ptsto_set_valid in H.
     repeat deex.
     congruence.
@@ -54,12 +53,18 @@ Proof.
     repeat deex.
     repeat inv_option. eauto.
   - right. eexists; intuition eauto.
-  - apply IHexec; auto.
-    (* XXX the sync-everything model is problematic because it means we have to
-     * restrict frame predicates.. *)
 Qed.
 
 Hint Extern 1 ({{_}} progseq (Read _) _) => apply read_ok : prog.
+
+Lemma ptsto_set_upd : forall a v v0 F m,
+  (a |=> v0 * F)%pred m -> (a |=> v * F)%pred (upd m a v).
+Proof.
+  unfold ptsto_set; intros.
+  destruct_lift H.
+  assert ((a |-> v * F)%pred (upd m a v)) by ( eapply ptsto_upd; eauto ).
+  destruct v; pred_apply; cancel.
+Qed.
 
 Theorem write_ok:
   forall (a:addr) (v:valu),
@@ -84,16 +89,49 @@ Proof.
     rewrite H3 in H8. inversion H8; subst.
     eapply pimpl_trans; [ apply pimpl_refl | | ].
     apply pimpl_sep_star; [ | apply pimpl_refl ].
-    eapply ptsto_incl.
     unfold valuset_list.
-    instantiate (l := (fst x :: x1)).
+    apply ptsto_incl.
     apply incl_cons; [ constructor; auto | ].
-    apply incl_tl; auto.
-    eapply ptsto_upd; eauto.
+    apply incl_tl; eauto.
+    eapply ptsto_set_upd; eauto.
   - right. eexists; intuition eauto.
 Qed.
 
 Hint Extern 1 ({{_}} progseq (Write _ _) _) => apply write_ok : prog.
+
+Theorem sync_ok:
+  forall (a:addr),
+  {< v,
+  PRE    a |=> v
+  POST:r a |=> (fst v, nil)
+  CRASH  a |=> v
+  >} Sync a.
+Proof.
+  unfold corr2, exis; intros; repeat deex.
+  destruct_lift H.
+  destruct x; simpl in *; subst.
+  inv_exec.
+  - apply sep_star_comm in H; apply ptsto_set_valid in H.
+    repeat deex.
+    congruence.
+  - eapply H4; eauto.
+    apply sep_star_and2lift; split; firstorder.
+    apply sep_star_and2lift; split; firstorder.
+    apply sep_star_comm.
+
+    apply sep_star_comm in H as H'.
+    apply ptsto_set_valid in H'.
+    destruct H'; destruct H0.
+    rewrite H6 in H0.
+    inversion H0; simpl in *; subst.
+
+    eapply ptsto_set_upd.
+    apply sep_star_comm.
+    eauto.
+  - right. eexists; intuition eauto.
+Qed.
+
+Hint Extern 1 ({{_}} progseq (Sync _ _) _) => apply sync_ok : prog.
 
 Definition If_ T P Q (b : {P} + {Q}) (p1 p2 : prog T) :=
   if b then p1 else p2.
@@ -137,8 +175,8 @@ Qed.
 Definition For_ (T: Set)
                 (L : Set) (G : Type) (f : addr -> L -> (L -> prog T) -> prog T)
                 (i n : addr) (l : L)
-                (nocrash : G -> addr -> L -> @pred valu)
-                (crashed : G -> @pred valu)
+                (nocrash : G -> addr -> L -> @pred valuset)
+                (crashed : G -> @pred valuset)
                 (rx: L -> prog T) : prog T.
   refine (Fix (@for_args_wf L) (fun _ => prog T)
           (fun args For_ => _)
